Added struct, missing some proofs

ulib/experimental/Steel.PCM.ArrayStruct.Memory.fst
@@ -15,6 +15,8 @@
 *)
 module Steel.PCM.ArrayStruct.Memory
 module U32 = FStar.UInt32
+module Univ = FStar.Universe
+module DepMap = FStar.DependentMap
 
 open FStar.FunctionalExtensionality
 open Steel.PCM
@@ -24,24 +26,59 @@ let v_usize = U32.v
 
 //TODO: use Steel.SizeT
 
-#set-options "--fuel 1 --ifuel 1"
+#set-options "--fuel 1 --ifuel 1 --print_universes"
+
+type field_id = string
 
 noeq type array_struct_descriptor : Type u#(a+1) =
+  // You can store your own funky PCM in the Base case
   | Base: a: Type u#a -> pcm: pcm a -> array_struct_descriptor
   | Array: t:array_struct_descriptor u#a -> len:usize -> array_struct_descriptor
+  | Struct: field_descriptors: (field_id ^-> option (array_struct_descriptor u#a)) ->
+    array_struct_descriptor
+  // Missing: untagged unions (not must have)
 
-let rec array_struct_type (descriptor: array_struct_descriptor) : Tot Type (decreases descriptor) =
+
+let rec array_struct_type (descriptor: array_struct_descriptor u#a) : Tot (Type u#a) (decreases descriptor) =
   match descriptor with
   | Base a pcm -> a
   | Array descriptor' len ->
     let type' = array_struct_type descriptor' in
     Seq.lseq type' (v_usize len)
+  | Struct field_descriptors ->
+    DepMap.t field_id (fun field_id -> match field_descriptors field_id with
+      | Some descr ->
+        FStar.WellFounded.axiom1 field_descriptors field_id;
+        array_struct_type descr
+      | None -> Univ.raise_t u#0 u#a False)
 
 noeq type array_struct : Type u#(a+1) =
   | ArrayStruct:
     descriptor: array_struct_descriptor u#a ->
-    value:(array_struct_type descriptor) ->
-    array_struct
+    value:(array_struct_type  descriptor) -> array_struct
+
+let field_type
+  (s: array_struct u#a{Struct? s.descriptor})
+  (field: field_id)
+    : Tot (Type u#a) =
+  match (Struct?.field_descriptors s.descriptor) field with
+  | Some descr ->
+    array_struct_type descr
+  | None -> Univ.raise_t u#0 u#a False
+
+let field_type_unroll_lemma
+  (s: array_struct u#a{Struct? s.descriptor})
+  (field: field_id)
+  : Lemma (DependentMap.t field_id (field_type s) == array_struct_type s.descriptor)
+  =
+  let open FStar.Tactics in
+  // TODO: prove that using some kind of normalization ?
+  admit();
+  assert (DependentMap.t field_id (field_type s) == array_struct_type s.descriptor) by begin
+    norm [delta_only ["Steel.PCM.ArrayStruct.Memory.field_type"]];
+    // TODO: how to unroll array_struct_type recursive definition here? zeta(_full) does not work
+    fail "HERE"
+  end
 
 let rec composable_array_struct' (s0 s1: array_struct) : Tot prop (decreases s0.descriptor) =
   match s0.descriptor, s1.descriptor with
@@ -57,8 +94,25 @@ let rec composable_array_struct' (s0 s1: array_struct) : Tot prop (decreases s0.
       let sub_s1 = ArrayStruct descriptor1 val1 in
       composable_array_struct' sub_s0 sub_s1
     end
+  | Struct field_descriptors0, Struct field_descriptors1 ->
+    field_descriptors0 == field_descriptors1 /\ begin forall (field: field_id). begin
+      match field_descriptors0 field, field_descriptors1 field with
+      | Some sub_descriptor0, Some sub_descriptor1 ->
+        field_type_unroll_lemma s0 field;
+        let v0 : DependentMap.t field_id (field_type s0) = s0.value in
+        let sub_v0 = DepMap.sel #_ #(field_type s0) v0 field in
+        field_type_unroll_lemma s1 field;
+        let v1 : DependentMap.t field_id (field_type s1) = s1.value in
+        let sub_v1 = DepMap.sel #_ #(field_type s1) v1 field in
+        let sub_s0 = ArrayStruct sub_descriptor0 sub_v0 in
+        let sub_s1 = ArrayStruct sub_descriptor1 sub_v1 in
+         FStar.WellFounded.axiom1 field_descriptors0 field;
+        composable_array_struct' sub_s0 sub_s1
+      | None, None -> True
+    end end
   | _ -> False
 
+#push-options "--warn_error -271"
 let rec composable_sym (s0 s1: array_struct)
     : Lemma
       (requires True)
@@ -105,6 +159,45 @@ let rec composable_sym (s0 s1: array_struct)
       Classical.forall_intro aux
     in
     Classical.impl_intro aux
+  | Struct field_descriptors0, Struct field_descriptors1 ->
+    let aux (_ : squash (composable_array_struct' s0 s1))
+       : Lemma (composable_array_struct' s1 s0) =
+      let aux' (field: field_id) : Lemma (
+        match field_descriptors0 field, field_descriptors1 field with
+        | Some sub_descriptor0, Some sub_descriptor1 ->
+          field_type_unroll_lemma s0 field;
+          let v0 : DependentMap.t field_id (field_type s0) = s0.value in
+          let sub_v0 = DepMap.sel #_ #(field_type s0) v0 field in
+          field_type_unroll_lemma s1 field;
+          let v1 : DependentMap.t field_id (field_type s1) = s1.value in
+          let sub_v1 = DepMap.sel #_ #(field_type s1) v1 field in
+          let sub_s0 = ArrayStruct sub_descriptor0 sub_v0 in
+          let sub_s1 = ArrayStruct sub_descriptor1 sub_v1 in
+          FStar.WellFounded.axiom1 field_descriptors0 field;
+          composable_array_struct' sub_s0 sub_s1
+        | None, None -> True
+      ) =
+        match field_descriptors0 field, field_descriptors1 field with
+        | Some sub_descriptor0, Some sub_descriptor1 ->
+          field_type_unroll_lemma s0 field;
+          let v0 : DependentMap.t field_id (field_type s0) = s0.value in
+          let sub_v0 = DepMap.sel #_ #(field_type s0) v0 field in
+          field_type_unroll_lemma s1 field;
+          let v1 : DependentMap.t field_id (field_type s1) = s1.value in
+          let sub_v1 = DepMap.sel #_ #(field_type s1) v1 field in
+          let sub_s0 = ArrayStruct sub_descriptor0 sub_v0 in
+          let sub_s1 = ArrayStruct sub_descriptor1 sub_v1 in
+          FStar.WellFounded.axiom1 field_descriptors0 field;
+          composable_sym sub_s1 sub_s0
+        | None, None -> ()
+      in
+      admit();
+      //TODO: why is the forall_intro not working?
+      Classical.forall_intro aux';
+      admit()
+    in
+    Classical.impl_intro aux;
+    assume(composable_array_struct' s1 s0 ==> composable_array_struct' s0 s1)
   | _ -> ()
 
 let composable_array_struct : symrel array_struct =
@@ -133,8 +226,10 @@ let rec compose_array_struct
       )
     in
     ArrayStruct s0.descriptor new_val
+  | Struct field_descriptors0, Struct field_descriptors1 ->
+    admit()
 
-let one_pcm : pcm unit = {
+let unit_pcm : pcm unit = {
   p = {
     composable = (fun () () -> True);
     op = (fun () () -> ());
@@ -146,7 +241,7 @@ let one_pcm : pcm unit = {
   is_unit = (fun _ -> ())
 }
 
-let one_array_struct = ArrayStruct (Base unit one_pcm) ()
+let one_array_struct = ArrayStruct (Base unit unit_pcm) ()
 
 let array_struct_pcm' : pcm' array_struct = {
   composable = composable_array_struct;
